LeanSAT/CNF.lean
@@ -4,5 +4,6 @@ Released under Apache 2.0 license as described in the file LICENSE.
 Authors: Henrik Böving
 -/
 import LeanSAT.CNF.Basic
+import LeanSAT.CNF.Literal
 import LeanSAT.CNF.Relabel
 import LeanSAT.CNF.RelabelFin
